Premier jet de F01, compilez avec 'make all doc'

coq2html/coqjs.js
@@ -1,0 +1,35 @@
+var trans_time = 500;
+
+/** Proofs are code blocks beginning with "Proof" */
+var proofs = $("span:contains('Proof')").parent('.code');
+
+/** Hides a proof and show a button */
+function hideProof(p, t) {
+    var link = $('<input type="button" value="Afficher la preuve"/>');
+    link.click(function() {
+        showProof(p, trans_time);
+        $(this).remove();
+    })
+    p.before(link);
+    p.slideUp(t);
+}
+
+/** Shows a proof and show a button */
+function showProof(p, t) {
+    var link = $('<input type="button" value="Masquer la preuve"/>');
+    link.click(function() {
+        hideProof(p, trans_time);
+        $(this).remove();
+    })
+    p.before(link);
+    p.slideDown(t);
+}
+
+/** Hide all proofs */
+function hideThemAll(p){
+    p.each(function() {
+        hideProof($(this), 0);
+    });
+}
+
+hideThemAll(proofs);
