Makefile
@@ -4,8 +4,8 @@ all:
 doc:
 	rm -rf html
 	mkdir html
-	coqdoc -utf8 -g -d html -s -toc F00_docindex.v F01_Defs.v F03_Insert_kind.v F04_Env_subst.v F05_Remove_var.v F06_Regularity.v F02_Inference.v 
-	cp -f coq2html/coqdoc.css html
+	coqdoc -utf8 -d html -s -toc F00_docindex.v F01_Defs.v F03_Insert_kind.v F04_Env_subst.v F05_Remove_var.v F06_Regularity.v F02_Inference.v 
+	cp -f coq2html/coqdoc.css coq2html/coqjs.js html
 
 coq2html/coq2html:
 	ocamllex coq2html/coq2html.mll
